

Zad 9 / Zestaw 2 Kinga Kondraciuk

$$\begin{cases} x_1 x_2 - x_1 = 2 \\ x_1^2 - x_2^2 = 1 \end{cases}$$

$$x_1 = -0,6$$

$$x_2 = -0,65$$

$$F(x_1, x_2) = \begin{bmatrix} x_1 x_2 - x_1 & -2 \\ x_1^2 - x_2^2 & -1 \end{bmatrix}$$

$$J(x_1, x_2) = \begin{bmatrix} \frac{\partial f_1}{\partial x_1} & \frac{\partial f_1}{\partial x_2} \\ \frac{\partial f_2}{\partial x_1} & \frac{\partial f_2}{\partial x_2} \end{bmatrix}$$

$$\frac{\partial f_1}{\partial x_1} = x_2 - 1$$

$$\frac{\partial f_1}{\partial x_2} = x_1$$

$$\frac{\partial f_2}{\partial x_1} = 2x_1$$

$$\frac{\partial f_2}{\partial x_2} = -2x_2$$

$$J(x_1, x_2) = \begin{bmatrix} x_2 - 1 & x_1 \\ 2x_1 & -2x_2 \end{bmatrix}$$

$$F(x^{(0)}) = \begin{bmatrix} -0,6(-0,65) - (-0,6) - 2 \\ (-0,6)^2 - (-0,65)^2 - 1 \end{bmatrix} = \begin{bmatrix} -1,01 \\ -1,0625 \end{bmatrix}$$

$$J(x^{(0)}) = \begin{bmatrix} -0,65-1 & -0,6 \\ 2(-0,6) & -2(-0,65) \end{bmatrix} = \begin{bmatrix} -1,65 & -0,60 \\ -1,2 & 1,3 \end{bmatrix}$$

$$x^{(k+1)} = x^{(k)} - (J(x^{(k)}))^{-1} F(x^{(k)})$$

$$J(x^{(0)})^{-1} = \frac{1}{-2,865} \begin{bmatrix} 1,3 & 0,6 \\ 1,2 & -1,65 \end{bmatrix} = \begin{bmatrix} -0,4538 & -0,2094 \\ -0,4188 & 0,5759 \end{bmatrix}$$

$$(J^{-1}F)(x^{(0)}) = \begin{bmatrix} 0,6808 \\ -0,1889 \end{bmatrix}$$

$$x^{(1)} = x^{(0)} - (J^{-1}F)(x^{(0)}) = \begin{bmatrix} -0,6 \\ -0,65 \end{bmatrix} - \begin{bmatrix} 0,6808 \\ -0,1889 \end{bmatrix} = \begin{bmatrix} -1,2808 \\ -0,4611 \end{bmatrix}$$

$$F(x^{(1)}) = \begin{bmatrix} -1,2808 \cdot (-0,4611) - (-1,2808) - 2 \\ (-1,2808)^2 - (-0,4611)^2 - 1 \end{bmatrix} = \begin{bmatrix} -0,1283 \\ 0,4278 \end{bmatrix}$$

$$J(x^{(1)}) = \begin{bmatrix} -1,461 & -1,281 \\ -2,561 & 0,9223 \end{bmatrix}$$

$$(J(x^{(1)}))^{-1} F(x^{(1)}) = \begin{bmatrix} -0,09277 \\ 0,2062 \end{bmatrix}$$

$$x^{(2)} = x^{(1)} - (J^{-1} F)(x^{(1)}) = \begin{bmatrix} -1,2808 \\ -0,4611 \end{bmatrix} - \begin{bmatrix} -0,09277 \\ 0,2062 \end{bmatrix} = \begin{bmatrix} -1,188 \\ -0,6673 \end{bmatrix}$$

$$F(x^{(2)}) = \begin{bmatrix} -0,01913 \\ -0,03392 \end{bmatrix}$$

$$J(x^{(2)}) = \begin{bmatrix} -1,667 & -1,189 \\ -2,376 & 1,335 \end{bmatrix}$$

$$(J(x^{(2)}))^{-1} F(x^{(2)}) = \begin{bmatrix} -0,01304 \\ 0,0024 \end{bmatrix}$$

$$x^{(3)} = x^{(2)} - (J^{-1} F)(x^{(2)}) = \begin{bmatrix} -1,201 \\ -0,6651 \end{bmatrix}$$

$$F(x^{(3)}) = \begin{bmatrix} -2,868 \cdot 10^{-5} \\ 1,652 \cdot 10^{-4} \end{bmatrix}$$

$$J(x^{(3)}) = \begin{bmatrix} -1,665 & -1,201 \\ -2,402 & 1,33 \end{bmatrix}$$

$$(J(x^{(3)}))^{-1} F(x^{(3)}) = \begin{bmatrix} 3,142 \cdot 10^{-5} \\ -6,745 \cdot 10^{-5} \end{bmatrix}$$

$$x^{(4)} = x^{(3)} + (J^{-1}F)(x^{(3)}) = \begin{bmatrix} -1,201 \\ -0,6652 \end{bmatrix}$$

$$F(x^{(4)}) = \begin{bmatrix} -2,12 \cdot 10^{-9} \\ -3,56 \cdot 10^{-9} \end{bmatrix}$$

Dokładności rzędu 10^{-9} , można zakończyć iteracje ponieważ osiągnięto zadaną dokładność (10^{-8}).